lib/ext.fst
@@ -1,0 +1,20 @@
+module Extensionality
+
+type arr (a:Type) (b:(a->Type)) = x:a -> Tot (b x)
+
+assume type Eq : #a:Type -> #b:(a -> Type) -> arr a b -> arr a b -> Type
+
+assume EqDef : forall (a:Type) (b:(a->Type)) (f:arr a b) (g:arr a b).
+              {:pattern Eq f g} (Eq f g) <==> (forall x. f x = g x)
+(*
+WARNING: '=' cannot be used in patterns.
+WARNING: '=' cannot be used in patterns.
+WARNING: 'and' cannot be used in patterns.
+WARNING: '=>' cannot be used in patterns.
+WARNING: '=' cannot be used in patterns.
+WARNING: '=>' cannot be used in patterns.
+WARNING: 'and' cannot be used in patterns.
+*)
+
+assume Extensionality : forall (a:Type) (b:(a->Type)) (f: arr a b) (g: arr a b).
+                        {:pattern Eq f g} Eq f g <==> f=g
